\section{Additional Exercises}\label{sec:MoreFunctionExercises}

\Opensolutionfile{solutions}[ex]
%%%%%%%%%%%%%%%%%%%%%%%%%%%%%%%%%%%%%%%%%%%%

\begin{enumialphparenastyle}

%%%%%%%%%%
\begin{ex}
Find the derivatives of the following functions
from definition.
\begin{enumerate}
	\item	$f(x)=(2x+3)^2$
	\item	$g(x)=x^{3/2}$
\end{enumerate}
\begin{sol}
\begin{enumerate}
	\item	$4(2x+3)$
	\item	$\frac{3}{2}x^{1/2}$
\end{enumerate}
\end{sol}
\end{ex}

%%%%%%%%%%
\begin{ex}
Let $f(x)=\left\{ 
\begin{array}{cc}
x^{3} & \text{if }x\leq 1 \\ 
5x-x^{2} & \text{if }x>1%
\end{array}%
\right. .$
Use the definition of the derivative to find $f^{\prime}(1)$.
\begin{sol}
	3
\end{sol}
\end{ex}

%%%%%%%%%%
\begin{ex}
Differentiate the following functions.
\begin{enumerate}
	\item	$y=7x^4-7\pi^4+\dfrac{1}{\pi\sqrt[3]{x}}$
	\item	$f(x)=\dfrac{1-\sqrt{x}}{1+\sqrt{x}}$
	\item	$f(x)=\vert x-1\vert+\vert x+2\vert$
	\item	$f(x)=x^2\sin x\cos x$
	\item	$y=\dfrac{x\sin x}{1+\sin x}$
	\item	$g(x)=\sqrt{2+\dfrac{3}{\sqrt{x}}}$
	\item	$y=\sqrt[3]{x^4+x^2+1}+\dfrac{1}{(x^3-x+4)^5}$
	\item	$y=\sin^3 x-\sin(x^3)$
	\item	$F(x)=\sec^4 x+\tan^4 x$
	\item	$y=\cos^2\left(\dfrac{1-x}{1+x}\right)$
	\item	$y=\tan(\sin(x^2+\sec^2 x))$
	\item	$y=\dfrac{1}{2+\sin\frac{\pi}{x}}$
\end{enumerate}
\begin{sol}
\begin{enumerate}
	\item	$28x^3-\dfrac{1}{3\pi x^{4/3}}$
	\item	$-\dfrac{1}{\sqrt{x}(1+\sqrt{x})^2}$
	\item	$f^{\prime}(x)=\left\{ 
	\begin{array}{ll}
	-2 & \text{if }x<-2 \\ 
	0 & \text{if }-2<x<1 \\ 
	2 & \text{if }x>1%
	\end{array}%
	\right. $
	\item	$2x\sin x\cos x+x^2\cos^2 x-x^2\sin^2 x$
	\item	$\dfrac{(\sin x+x\cos x)(1+\sin x)-x\sin x\cos x}{(1+\sin x)^2}$
	\item	$-\dfrac{3}{4x^{3/2}}\left(2+\dfrac{3}{\sqrt{x}}\right)^{-1/2}$
	\item	$\frac{1}{3}(x^4+x^2+1)^{-2/3}(4x^3+2x)-\dfrac{5(3x^2-1)}{(x^3-x+4)^6}$
	\item	$3\sin^2 x\cos x-3x^2\cos(x^3)$
	\item	$4\sec^4 x\tan x + 4\tan^3 x\sec^2 x$
	\item	$\dfrac{4}{(1+x)^2}\cos\left(\dfrac{1-x}{1+x}\right)\sin\left(\dfrac{1-x}{1+x}\right)$
	\item	$(2x+2\sec^2 x\tan x)\sec^2(\sin(x^2+\sec^2 x))\cos(x^2+\sec^2 x)$
	\item	$-\dfrac{\pi\cos\frac{\pi}{x}}{x^2(2+\sin\frac{\pi}{x})^2}$
\end{enumerate}
\end{sol}
\end{ex}

%%%%%%%%%%
\begin{ex}
Differentiate the following functions.
\begin{enumerate}
	\item	$y=e^{3x}+e^{-x}+e^2$
	\item	$y=e^{2x}\cos 3x$
	\item	$f(x)=\tan(x+e^x)$
	\item	$g(x)=\dfrac{e^x}{e^x+2}$
	\item	$y=\ln(2+\sin x)-\sin(2+\ln x)$
	\item	$f(x)=e^{x^{\pi}}+x^{\pi^{e}}+\pi^{e^x}$
	\item	$y=\log _{a}(b^x)+b^{\log_a x}$, where $a$ and $b$ are positive real numbers and $a\neq 1$
	\item	$y=(x^2+1)^{x^3+1}$
	\item	$y=(x^2+e^x)^{1/\ln x}$
	\item	$y=\dfrac{x\sqrt{x^2+x+1}}{(2+\sin x)^4(3x+5)^7}$
\end{enumerate}
\begin{sol}
\begin{enumerate}
	\item	$3e^{3x}-e^{-x}$
	\item	$2e^{2x}\cos 3x-3e^{2x}\sin 3x$
	\item	$(1+e^x)\sec^2(x+e^x)$
	\item	$2e^x/(e^x+2)^2$
	\item	$\dfrac{\cos x}{2+\sin x}-\dfrac{\cos(2+\ln	x)}{x}$
	\item	$e^{x^{\pi}}\cdot\pi x^{\pi-1}+\pi^e x^{\pi^e-1}+\pi^{e^x}\ln\pi\cdot e^x$
	\item	$\log_{a}b+(\log_{a}b) x^{(\log_{a}b)-1}$
	\item	$(x^2+1)^{x^3+1}\left(3x^2\ln(x^2+1)+\dfrac{2x(x^3+1)}{x^2+1}\right)$
	\item	$\dfrac{(x^2+e^x)^{1/\ln x}}{(\ln x)^2}\left(\dfrac{2x+e^x}{x^2+e^x}\ln	x-\dfrac{x^2+e^x}{x}\right)$
	\item	$\dfrac{x\sqrt{x^2+x+1}}{(2+\sin x)^4 (3x+5)^7} \left(\dfrac{1}{x}+\dfrac{2x+1}{2(x^2+x+1)}-\dfrac{4\cos x}{2+\sin x}-\dfrac{21}{3x+5}\right)$
\end{enumerate}
\end{sol}
\end{ex}

%%%%%%%%%%
\begin{ex}
Find $\dfrac{dy}{dx}$ if $y$ is a differentiable
function that satisfy the given equation.
\begin{enumerate}
	\item	$x^2+xy+y^2=7$
	\item	$x^2+y^2=(2x^2+2y^2-x)^2$
	\item	$x^2\sin y+y^3=\cos x$
	\item	$x^2+xe^y=2y+e^x$
\end{enumerate}
\begin{sol}
\begin{enumerate}
	\item	$-(2x+y)/(x+2y)$
	\item	$\dfrac{x-(2x^2+2y^2-x) (4x-1)}{4y(2x^2+2y^2-x)-y}$
	\item	$-\dfrac{\sin x+2x\sin y}{x^2\cos y+3y^2}$
	\item	$\dfrac{2x+e^y-e^x}{2-xe^y}$
\end{enumerate}
\end{sol}
\end{ex}

%%%%%%%%%%
\begin{ex}
Differentiate the following functions.
\begin{enumerate}
	\item	$y=x\sin^{-1}x$
	\item	$f(x)=\dfrac{\sin^{-1}x}{\cos^{-1}x}$
	\item	$g(x)=\tan^{-1}\left(\dfrac{x}{a}\right)$, where $a>0$
	\item	$y=x\tan^{-1}x-\dfrac{1}{2}\ln(x^2+1)$
\end{enumerate}
\begin{sol}
\begin{enumerate}
	\item	$\sin^{-1}x+x/\sqrt{1-x^2}$
	\item	$\dfrac{\cos^{-1}x+\sin^{-1}x}{(\cos^{-1}x)^2 \sqrt{1-x^2}}$
	\item	$a/(x^2+a^2)$
	\item	$\tan^{-1}x$
\end{enumerate}
\end{sol}
\end{ex}


\end{enumialphparenastyle}