\subsection{Law of Exponents}
The Law of Exponents is a set of rules for simplifying expressions that governs 
the combination of exponents (powers).
Recall that $\sqrt[n]{~}$ denotes the $n$th root. 
For example $\sqrt[3]{8}=2$ represents that the cube root of $8$ is equal to $2$.\\

\begin{definition}{Law of Exponents}{ExponentRules1}
{\bf Definitions}

If $m,n$ are positive integers, then:
\begin{multicols}{2}
\begin{enumerate}
	\item $x^n=x\cdot x\cdot\ldots\cdot x$ ($n$ times).
	\item $x^0=1$, for $x\neq 0$.
	\item $\ds{x^{-n}=\frac{1}{x^n}}$, for $x\neq 0$.
	\item $x^{m/n}=\sqrt[n]{x^m}$ or $\left(\sqrt[n]{x}\right)^m$, for $x\geq 0$.
\end{enumerate}
\end{multicols}

{\bf Combining}
\begin{multicols}{3}
\begin{enumerate}
	\item $x^ax^b=x^{a+b}$.
	\item $\ds{\frac{x^a}{x^b}=x^{a-b}}$, for $x\neq 0$.
	\item $\left(x^a\right)^b=x^{ab}=x^{ba}=\left(x^b\right)^a$.
\end{enumerate}
\end{multicols}

{\bf Distributing}
\begin{multicols}{2}
\begin{enumerate}
	\item $(xy)^a=x^ay^a$, for $x\geq 0$, $y\geq 0$.
	\item $\ds{\left(\frac{x}{y}\right)^a=\frac{x^a}{y^a}}$, for $x\geq 0$, $y>0$.
\end{enumerate}
\end{multicols}
\end{definition}

In the next example, the word \ifont{simplify} means \ifont{to make simpler} or to write the expression more compactly.\\

\begin{example}{Laws of Exponents}{LawsExponents}\label{LawsExponents}
Simplify the following expression as much as possible assuming $x,y>0$:
$$\frac{3x^{-2}y^3x}{y^2\sqrt x}.$$
\vspace{-0.5cm}
\end{example}

\begin{solution}
Using the Law of Exponents, we have:
$$\def\arraystretch{2.5}
\begin{array}{>{\displaystyle}r>{\displaystyle}c>{\displaystyle}l>{\displaystyle}l}
\frac{3x^{-2}y^3x}{y^2\sqrt x} & = & \frac{3x^{-2}y^3x}{y^2x^{\frac{1}{2}}}, 
		&\mbox{since $\ds\sqrt x = x^{\frac{1}{2}}$},\\
~ & = & \frac{3x^{-2}yx}{x^{\frac{1}{2}}}, 
		&\mbox{since $\ds\frac{y^3}{y^2}=y$},\\
~ & = & \frac{3y}{x^{\frac{3}{2}}}, 
		&\mbox{since $\ds\frac{x^{-2}x}{x^{\frac{1}{2}}}=\frac{x^{-1}}{x^{\frac{1}{2}}} =x^{-\frac{3}{2}}=\frac{1}{x^{\frac{3}{2}}}$},\\
~ & = & \frac{3y}{\sqrt{x^3}}, 
		&\mbox{since $\ds x^{\frac{3}{2}}=\sqrt{x^3}$}.
\end{array}$$
An answer of $3yx^{-3/2}$ is equally acceptable, and such an expression may prove to be computationally simpler, although a positive exponent may be preferred.
\end{solution}
